theories/prob_eff_lang/probblaze/sem_row.v
@@ -11,33 +11,39 @@ From iris.base_logic Require Export iprop upred invariants.
 From clutch.prob_eff_lang.probblaze Require Import logic notation sem_def mode sem_sig.
 
 (* Nil Row *)
-Program Definition sem_row_nil {Σ} : sem_row Σ := @SemRow Σ ⊥ _. 
-Next Obligation. iIntros (????) "[]". Qed.
+Program Definition sem_row_nil {Σ} : sem_row Σ := @SemRow Σ ⊥ _ _. 
+Next Obligation. iIntros (?????) "? (%l1 & %l2 & %X & %Hcontra & ?)". by apply elem_of_nil in Hcontra. Qed.
+Next Obligation. iIntros (????) "(%l1 & %l2 & %X & %Hcontra & ?)". by apply elem_of_nil in Hcontra. Qed.
 
 Global Instance sem_row_bottom {Σ} : Bottom (sem_row Σ) := sem_row_nil.
-
+(* TODO: update to use iLblThy s.t. we can use BREL *)
 (* Cons Row *)
-Program Definition sem_row_cons {Σ} (op : label) : sem_sig Σ -d> sem_row Σ -d> sem_row Σ :=
-    λ σ ρ, (@SemRow Σ (@PMonoProt Σ ( 
-              (λ e1 e2, λne Φ, ∃ (op' : label) (v1 v2 : val), 
-                           ⌜ e1 = (do: op' v1)%E ⌝ ∗ ⌜ e2 = (do: op' v2)%E ⌝ ∗
-                            if decide (op = op') then 
-                              ▷ ((pmono_prot_car σ) v1 v2 Φ)
-                            else
-                              (pmono_prot_car (sem_row_car ρ)) (do: op' v1)%E (do: op' v2)%E Φ)%I) _) _).
-Next Obligation. 
-  intros ??????????. repeat f_equiv; done. 
+Program Definition sem_row_cons {Σ} (op1 op2 : label) : sem_sig Σ -d> sem_row Σ -d> sem_row Σ :=
+    λ σ ρ, (@SemRow Σ (@LblSig Σ ((([op1], [op2]), σ) :: (sem_row_car ρ))) _ _ ) .
+              (* (λ e1 e2, λne Φ, ∃ (op' : label) (v1 v2 : val), 
+                              ⌜ e1 = (do: op' v1)%E ⌝ ∗ ⌜ e2 = (do: op' v2)%E ⌝ ∗
+                               if decide (op = op') then 
+                                 ▷ ((pmono_prot_car σ) v1 v2 Φ)
+                               else
+                                 (pmono_prot_car (sem_row_car ρ)) (do: op' v1)%E (do: op' v2)%E Φ)%I) _). *)
+Next Obligation. intros ?????. iIntros (????) "#H1 H2". iApply to_iThy_cons. iDestruct (to_iThy_cons with "H2") as "H2".
+                 iDestruct "H2" as "[(%&%&%&%&%&->&%&->&%&Hσ&#Hcont)|(%&%&%&%&%&%&%&%&%&->&%&->&%&Hσ&#Hcont)]"; [iLeft|iRight].
+                 - iExists _,_,_,_,_. do 4 (iSplit; [iPureIntro;done|]). iFrame.
+                   iModIntro. iIntros (??) "HS". iDestruct ("Hcont" with "HS") as "HΦ".
+                   by iApply "H1".
+                 - simpl. iExists _,_,_. iFrame. iSplit; [iPureIntro; done|].
+                   iExists _,_. do 4 (iSplit;[iPureIntro;done|]).
+                   iIntros "!# % % HS". iDestruct ("Hcont" with "HS") as "HΦ".
+                   by iApply "H1".
 Qed.
 Next Obligation.
-  iIntros (????????) "#HPost (%op' & %v1' & %v2' & -> & -> & H)". simpl.
-  iExists op', v1', v2'. do 2 (iSplit; first done).
-  destruct (decide (op = op')).
-  - iApply (pmono_prot_prop Σ σ with "HPost H").
-  - iApply (pmono_prot_prop Σ ρ with "HPost H").
-Qed.
-Next Obligation.
-  iIntros (???????) "(%op' & %v1' & %v2' & -> & -> & H)". by iExists op', v1', v2'.
-Qed.
+  iIntros (????????) "H". 
+  iDestruct (to_iThy_cons with "H") as "H". 
+  iDestruct "H" as "[(%&%&%&%&%&->&%&->&%&Hσ&#Hcont)|(%&%&%&%&%&%&%&%&%&->&%&->&%&Hσ&#Hcont)]".
+  - destruct σ. iDestruct sem_sig_prop as "H1". iExists _, _.
+    iDestruct ("H1" with "Hσ") as (????) "H". iExists op0, op3, v1,v2.
+    iDestruct "H" as "(-> & ->)". done.
+  - Admitted.
 
 (* Recursive Row *)
 Definition sem_row_rec {Σ} (R : sem_row Σ → sem_row Σ) `{Contractive R} : sem_row Σ :=
@@ -47,25 +53,29 @@ Lemma sem_row_rec_unfold {Σ} (R : sem_row Σ → sem_row Σ) `{Contractive R} :
   sem_row_rec R ≡ R (sem_row_rec R).
 Proof. rewrite /sem_row_rec {1} fixpoint_unfold //. Qed.
 
-Lemma sem_row_rec_unfold_iThy {Σ} (R : sem_row Σ → sem_row Σ) `{Contractive R} e1 e2 Φ:
-  pmono_prot_car (sem_row_car (sem_row_rec R)) e1 e2 Φ ≡ pmono_prot_car (sem_row_car (R (sem_row_rec R))) e1 e2 Φ.
-Proof. f_equiv. apply non_dep_fun_equiv.  apply non_dep_fun_equiv. rewrite {1}sem_row_rec_unfold //. Qed.
+(* Lemma sem_row_rec_unfold_iThy {Σ} (R : sem_row Σ → sem_row Σ) `{Contractive R} e1 e2 Φ:
+     pmono_prot_car (sem_row_car (sem_row_rec R)) e1 e2 Φ ≡ pmono_prot_car (sem_row_car (R (sem_row_rec R))) e1 e2 Φ.
+   Proof. f_equiv. apply non_dep_fun_equiv.  apply non_dep_fun_equiv. rewrite {1}sem_row_rec_unfold //. Qed. *)
 
 (* Flip-Bang Row *)
+(* TOOD: Find a better way to make iLblSig a subtype of iLblThy -- the properties of the elements in the list are not preserved *)                          
+Definition iThyIfMono_iLblSig {Σ} (m: mode) (L : iLblSig Σ) : iLblSig Σ :=
+  @LblSig Σ (map (λ '(l1s, l2s, X), (l1s, l2s, sem_sig_flip_mbang m X)) L).
+
 Program Definition sem_row_flip_mbang {Σ} (m : mode) (ρ : sem_row Σ) : sem_row Σ := 
-  @SemRow Σ (@PMonoProt Σ (iThyIfMono m ρ) _) _.
+  @SemRow Σ (@LblSig Σ (iThyIfMono_iLblSig m ρ)) _ _.
 Next Obligation.
   iIntros (???????) "#HΦ Hσ". 
-  destruct m;simpl.
-  - iDestruct "Hσ" as (Q') "($ & Hpost)". iModIntro.
-    iIntros (??) "HQ'". iApply "HΦ". by iApply "Hpost".
-  - by iApply (pmono_prot_prop with "HΦ").
+  iDestruct "Hσ" as (????????? -> ? -> ?) "(HX & #Hcont)".
+  iExists _, _, _. iFrame. iSplit; [iPureIntro;done|].
+  iExists _,_. repeat (iSplit; [iPureIntro; done|]).
+  iIntros (??) "!# HS". iApply "HΦ". by iApply "Hcont".
 Qed.
 Next Obligation.
   iIntros (??????) "Hρ". destruct m.
-  - simpl. iDestruct "Hρ" as (?) "(Hρ & _)". iApply (sem_row_prop _ ρ with "Hρ").
-  - iApply (sem_row_prop _ ρ with "Hρ").
-Qed.
+  - simpl. iDestruct "Hρ" as (????????? -> ? -> ?) "(HX & #Hcont)". simpl in *. admit.
+  - simpl.
+Admitted.
 
 (* Notations. *)
 Notation "⟨⟩" := (sem_row_nil) : sem_row_scope.
@@ -112,159 +122,167 @@ Section once_row.
 
   (* Once Constraint *)
   
-  Class OnceR {Σ} (ρ : sem_row Σ) := {
+  Class OnceR `{probblazeRGS Σ} (ρ : sem_row Σ) := {
     row_le_mfbang_elim : (⊢ (¡ ρ%R) ≤ᵣ ρ%R)
   }.
-  
-  Global Instance monoprot_once {Σ} (ρ : sem_row Σ) `{! OnceR ρ } : MonoProt ρ.
+
+  (* TODO: figure out typeclasses to use OnceR *)
+  Global Instance monoprot_once `{probblazeRGS Σ} (ρ : sem_row Σ) `{! OnceR ρ } : MonoProt (to_iThy ρ).
   Proof.
     constructor. iIntros (????) "HP Hρ".
-    inv OnceR0. iApply row_le_mfbang_elim0.
-    iExists Φ. simpl. iFrame.
-  Qed.
-
+    inv OnceR0. (* iApply row_le_mfbang_elim0. *)
+  Admitted. 
 End once_row.
 
 Section row_sub_typing.
-
+  Context `{probblazeRGS Σ}.
   (* Subtyping on Rows *)
   
-  Lemma row_le_refl {Σ} (ρ : sem_row Σ) :
+  Lemma row_le_refl (ρ : sem_row Σ) :
     ⊢ ρ ≤ᵣ ρ.
-  Proof. iApply iThy_le_refl. Qed.
+  Proof. iApply to_iThy_le_refl. Qed.
   
-  Lemma row_le_trans {Σ} (ρ₁ ρ₂ ρ₃ : sem_row Σ) :
+  Lemma row_le_trans (ρ₁ ρ₂ ρ₃ : sem_row Σ) :
     ρ₁ ≤ᵣ ρ₂ -∗ 
     ρ₂ ≤ᵣ ρ₃ -∗
     ρ₁ ≤ᵣ ρ₃.
-  Proof. iApply iThy_le_trans. Qed.
+  Proof. iApply to_iThy_le_trans. Qed.
   
-  Lemma row_le_nil {Σ} (ρ : sem_row Σ) : 
+  Lemma row_le_nil (ρ : sem_row Σ) : 
     ⊢ ⟨⟩ ≤ᵣ ρ.
-  Proof. iApply iThy_le_bot. Qed.
+  Proof. iApply to_iThy_le_bot. Qed.
+
+  (* TODO: figure out how to extend sem_rows *)
+  (* Lemma row_le_cons_comp (ρ ρ' : sem_row Σ) (op op' : label) (σ σ' : sem_sig Σ) : 
+       σ ≤ₛ σ' -∗ ρ ≤ᵣ ρ' -∗ 
+       [([op], [op'], σ)] ⋅ ρ ≤ᵣ ([op], [op'], σ') · ρ'.
+     Proof.
+       iIntros "#Hσσ' #Hρρ'". rewrite /sem_row_cons /=. 
+       iIntros (???) "!# (%op' & %v1' & %v2' & -> & -> & H)".
+       iExists op', v1', v2'; do 2 (iSplit; first done).
+       destruct (decide (op = op')); first (by iApply "Hσσ'"). 
+       by iApply "Hρρ'".
+     Qed.
+     
+     Lemma row_le_swap_second {Σ} (op op' : label) (σ σ' : sem_sig Σ) (ρ : sem_row Σ) : 
+       op ≠ op' →
+       ⊢ (op, σ) · (op', σ') · ρ ≤ᵣ (op', σ') · (op, σ) · ρ. 
+     Proof. 
+       iIntros (Hneq). rewrite /sem_row_cons /=.
+       iIntros (???) "!# (%op'' & %v1'' & %v2'' & %Heq1 & %Heq2 & H)". simpl.
+       destruct (decide (op = op'')) as [->|].
+       - iExists op'', v1'', v2''. do 2 (iSplit; first done).
+         rewrite decide_False; last done.
+         iExists op'', v1'', v2''; do 2 (iSplit; first done).
+         rewrite decide_True //.
+       - iDestruct "H" as "(%op''' & %v1''' & %v2''' & %Heq1' & %Heq2' & H)".
+         destruct (decide (op' = op''')) as [->|].
+         + iExists op'', v1'', v2''; do 2 (iSplit; first done).
+           simplify_eq. rewrite decide_True //.
+         + iExists op''', v1'', v2''; do 2 (iSplit; first by simplify_eq).
+           simplify_eq. rewrite decide_False //.
+           iExists op''', v1''', v2'''. do 2 (iSplit; first done).
+           rewrite decide_False //.
+     Qed.
+     
+     Corollary row_le_swap_third {Σ} (op op' op'' : label) (σ σ' σ'' : sem_sig Σ) (ρ : sem_row Σ) : 
+       op ≠ op' → op' ≠ op'' → op'' ≠ op →
+       ⊢ (op, σ) · (op', σ') · (op'', σ'') · ρ ≤ᵣ (op'', σ'') · (op, σ) · (op', σ') · ρ. 
+     Proof. 
+       iIntros (???). 
+       iApply row_le_trans; first iApply row_le_cons_comp; [iApply sig_le_refl|by iApply row_le_swap_second|].
+       by iApply row_le_swap_second.
+     Qed.
+     
+     Corollary row_le_swap_fourth {Σ} (op op' op'' op''' : label) (σ σ' σ'' σ''': sem_sig Σ) (ρ : sem_row Σ) : 
+       op ≠ op' → op ≠ op'' → op ≠ op''' → op' ≠ op'' → op' ≠ op''' → op'' ≠ op''' → 
+       ⊢ (op, σ) · (op', σ') · (op'', σ'') · (op''', σ''') · ρ ≤ᵣ 
+         (op''', σ''') · (op, σ) · (op', σ') · (op'', σ'') · ρ.
+     Proof. 
+       iIntros (??????). 
+       iApply row_le_trans; first iApply row_le_cons_comp; [iApply sig_le_refl|by iApply row_le_swap_third|].
+       by iApply row_le_swap_second.
+     Qed. *)
   
-  Lemma row_le_cons_comp {Σ} (ρ ρ' : sem_row Σ) (op : label) (σ σ' : sem_sig Σ) : 
-    σ ≤ₛ σ' -∗ ρ ≤ᵣ ρ' -∗ 
-    (op, σ) · ρ ≤ᵣ (op, σ') · ρ'.
-  Proof.
-    iIntros "#Hσσ' #Hρρ'". rewrite /sem_row_cons /=. 
-    iIntros (???) "!# (%op' & %v1' & %v2' & -> & -> & H)".
-    iExists op', v1', v2'; do 2 (iSplit; first done).
-    destruct (decide (op = op')); first (by iApply "Hσσ'"). 
-    by iApply "Hρρ'".
-  Qed.
-  
-  Lemma row_le_swap_second {Σ} (op op' : label) (σ σ' : sem_sig Σ) (ρ : sem_row Σ) : 
-    op ≠ op' →
-    ⊢ (op, σ) · (op', σ') · ρ ≤ᵣ (op', σ') · (op, σ) · ρ. 
-  Proof. 
-    iIntros (Hneq). rewrite /sem_row_cons /=.
-    iIntros (???) "!# (%op'' & %v1'' & %v2'' & %Heq1 & %Heq2 & H)". simpl.
-    destruct (decide (op = op'')) as [->|].
-    - iExists op'', v1'', v2''. do 2 (iSplit; first done).
-      rewrite decide_False; last done.
-      iExists op'', v1'', v2''; do 2 (iSplit; first done).
-      rewrite decide_True //.
-    - iDestruct "H" as "(%op''' & %v1''' & %v2''' & %Heq1' & %Heq2' & H)".
-      destruct (decide (op' = op''')) as [->|].
-      + iExists op'', v1'', v2''; do 2 (iSplit; first done).
-        simplify_eq. rewrite decide_True //.
-      + iExists op''', v1'', v2''; do 2 (iSplit; first by simplify_eq).
-        simplify_eq. rewrite decide_False //.
-        iExists op''', v1''', v2'''. do 2 (iSplit; first done).
-        rewrite decide_False //.
-  Qed.
-  
-  Corollary row_le_swap_third {Σ} (op op' op'' : label) (σ σ' σ'' : sem_sig Σ) (ρ : sem_row Σ) : 
-    op ≠ op' → op' ≠ op'' → op'' ≠ op →
-    ⊢ (op, σ) · (op', σ') · (op'', σ'') · ρ ≤ᵣ (op'', σ'') · (op, σ) · (op', σ') · ρ. 
-  Proof. 
-    iIntros (???). 
-    iApply row_le_trans; first iApply row_le_cons_comp; [iApply sig_le_refl|by iApply row_le_swap_second|].
-    by iApply row_le_swap_second.
-  Qed.
-  
-  Corollary row_le_swap_fourth {Σ} (op op' op'' op''' : label) (σ σ' σ'' σ''': sem_sig Σ) (ρ : sem_row Σ) : 
-    op ≠ op' → op ≠ op'' → op ≠ op''' → op' ≠ op'' → op' ≠ op''' → op'' ≠ op''' → 
-    ⊢ (op, σ) · (op', σ') · (op'', σ'') · (op''', σ''') · ρ ≤ᵣ 
-      (op''', σ''') · (op, σ) · (op', σ') · (op'', σ'') · ρ.
-  Proof. 
-    iIntros (??????). 
-    iApply row_le_trans; first iApply row_le_cons_comp; [iApply sig_le_refl|by iApply row_le_swap_third|].
-    by iApply row_le_swap_second.
-  Qed.
-  
-  Lemma row_le_rec_unfold {Σ} (R : sem_row Σ → sem_row Σ) `{Contractive R} :
+  Lemma row_le_rec_unfold (R : sem_row Σ → sem_row Σ) `{Contractive R} :
     ⊢ (μᵣ θ, R θ) ≤ᵣ R (μᵣ θ, R θ).
   Proof. rewrite {1} sem_row_rec_unfold //. iApply row_le_refl. Qed.
   
-  Lemma row_le_rec_fold {Σ} (R : sem_row Σ → sem_row Σ) `{ Contractive R }:
+  Lemma row_le_rec_fold (R : sem_row Σ → sem_row Σ) `{ Contractive R }:
     ⊢ R (μᵣ θ, R θ) ≤ᵣ (μᵣ θ, R θ).
   Proof. rewrite - {1} sem_row_rec_unfold. iApply row_le_refl. Qed.
-  
-  Lemma row_le_mfbang_intro {Σ} (m : mode) (ρ : sem_row Σ) :
+
+  (* TODO: typeclasses... *)
+  Lemma row_le_mfbang_intro (m : mode) (ρ : sem_row Σ) :
     ⊢ ρ ≤ᵣ ¡[ m ] ρ. 
   Proof. 
-    rewrite /sem_row_flip_mbang. iIntros (???) "!# Hρ". simpl.
-    destruct m; [|done]. simpl.
-    iExists Q. iFrame. iModIntro.
-    iIntros "% % $ //".
-  Qed.
-  
-  Lemma row_le_mfbang_elim_ms {Σ} (ρ : sem_row Σ) :
+  (*   rewrite /sem_row_flip_mbang. iIntros (???) "!# Hρ". simpl.
+       destruct m; [|done]. simpl.
+       iExists Q. iFrame. iModIntro.
+       iIntros "% % $ //".
+     Qed. *)
+  Admitted. 
+    
+  Lemma row_le_mfbang_elim_ms (ρ : sem_row Σ) :
     ⊢ ¡[MS] ρ ≤ᵣ ρ. 
   Proof. 
-    rewrite /sem_sig_flip_mbang. 
-    iIntros (v1 v2 Φ) "!# H". done. 
-  Qed.
-  
-  Lemma row_le_mfbang_comp {Σ} m m' (ρ ρ' : sem_row Σ) :
+    (* rewrite /sem_sig_flip_mbang. 
+       iIntros (v1 v2 Φ) "!# H". done. 
+     Qed. *)
+  Admitted. 
+
+  (* Lemma to_iThy_le_iThyIfMono_iLblSig (L M : iLblSig Σ) :
+       L ≤ᵣ M -∗ (iThyIfMono_iLblSig L) ≤ᵣ (iThyIfMono_iLblSig M). *)
+  (* TODO: proof a theorem like iThy_le_iThyMono for iThyIfMono_iLblSig *)
+  Lemma row_le_mfbang_comp m m' (ρ ρ' : sem_row Σ) :
     m' ≤ₘ m -∗ ρ ≤ᵣ ρ' -∗
     (¡[m] ρ) ≤ᵣ (¡[m'] ρ').
   Proof. 
-    iIntros "#Hlem #Hleσ". destruct m.
-    - iDestruct (mode_le_OS_inv with "Hlem") as "->".
-      rewrite /row_le /sem_row_flip_mbang /tc_opaque.
-      by iApply iThy_le_iThyMono.
-    - iApply row_le_trans; first iApply row_le_mfbang_elim_ms. 
-      iApply row_le_trans; first iApply (row_le_mfbang_intro m').
-      rewrite /row_le /sem_row_flip_mbang /tc_opaque.
-      by iApply iThy_le_iThyIfMono.
-  Qed.
+  (*   iIntros "#Hlem #Hleσ". destruct m.
+       - iDestruct (mode_le_OS_inv with "Hlem") as "->".
+         rewrite /row_le /sem_row_flip_mbang /tc_opaque.
+         by iApply iThy_le_iThyMono.
+       - iApply row_le_trans; first iApply row_le_mfbang_elim_ms. 
+         iApply row_le_trans; first iApply (row_le_mfbang_intro m').
+         rewrite /row_le /sem_row_flip_mbang /tc_opaque.
+         by iApply iThy_le_iThyIfMono.
+     Qed. *)
+  Admitted. 
   
-  Lemma row_le_mfbang_dist_cons {Σ} op m σ (ρ : sem_row Σ) :
-    ⊢ ¡[ m ] ((op, σ) · ρ) ≤ᵣ (op, ¡[ m ] σ)%S · (¡[ m ] ρ).
-  Proof. 
-    rewrite /sem_row_flip_mbang. iIntros (???) "!# H". simpl.
-    destruct m; simpl; [|done]. 
-    iDestruct "H" as (Q') "((%op' & %v1' & %v2' & -> & -> & H) & Hpost)".
-    iExists op', v1', v2'. do 2 (iSplit; first done).
-    destruct (decide (op = op')); first iNext; iExists Q'; iFrame. 
-  Qed.
-
-  Global Instance row_cons_once {Σ} (ρ : sem_row Σ) op (σ : sem_sig Σ) `{! OnceS σ, ! OnceR ρ } :
-    OnceR ((op, σ) · ρ)%R.
-  Proof.
-    constructor. inv OnceS0. inv OnceR0.
-    iApply row_le_trans; first iApply row_le_mfbang_dist_cons.
-    iApply row_le_cons_comp; [iApply sig_le_mfbang_elim|iApply row_le_mfbang_elim0].
-  Qed.
+  (* Lemma row_le_mfbang_dist_cons {Σ} op m σ (ρ : sem_row Σ) :
+       ⊢ ¡[ m ] ((op, σ) · ρ) ≤ᵣ (op, ¡[ m ] σ)%S · (¡[ m ] ρ).
+     Proof. 
+       rewrite /sem_row_flip_mbang. iIntros (???) "!# H". simpl.
+       destruct m; simpl; [|done]. 
+       iDestruct "H" as (Q') "((%op' & %v1' & %v2' & -> & -> & H) & Hpost)".
+       iExists op', v1', v2'. do 2 (iSplit; first done).
+       destruct (decide (op = op')); first iNext; iExists Q'; iFrame. 
+     Qed.
+     
+     Global Instance row_cons_once {Σ} (ρ : sem_row Σ) op (σ : sem_sig Σ) `{! OnceS σ, ! OnceR ρ } :
+       OnceR ((op, σ) · ρ)%R.
+     Proof.
+       constructor. inv OnceS0. inv OnceR0.
+       iApply row_le_trans; first iApply row_le_mfbang_dist_cons.
+       iApply row_le_cons_comp; [iApply sig_le_mfbang_elim|iApply row_le_mfbang_elim0].
+     Qed. *)
   
-  Lemma row_le_mfbang_idemp {Σ} m (ρ : sem_row Σ) :
+  Lemma row_le_mfbang_idemp m (ρ : sem_row Σ) :
     ⊢ (¡[ m ] (¡[ m ] ρ)) ≤ᵣ ((¡[ m ] ρ)).
-  Proof. 
-    iIntros (v1 v2 Φ) "!# H".
-    destruct m; [|done]. simpl.    
-    iDestruct "H" as (Q') "((%Q'' & Hρ & HPost') & HPost)". 
-    iExists Q''. iFrame. 
-    iIntros (??) "!> HQ''".
-    iApply "HPost". by iApply "HPost'".
-  Qed.
+  (* Proof. 
+       iIntros (v1 v2 Φ) "!# H".
+       destruct m; [|done]. simpl.    
+       iDestruct "H" as (Q') "((%Q'' & Hρ & HPost') & HPost)". 
+       iExists Q''. iFrame. 
+       iIntros (??) "!> HQ''".
+       iApply "HPost". by iApply "HPost'".
+     Qed. *)
+  Admitted. 
 
-  Global Instance row_fbang_once {Σ} (ρ : sem_row Σ) : OnceR (¡ ρ)%R.
+  Global Instance row_fbang_once (ρ : sem_row Σ) : OnceR (¡ ρ)%R.
   Proof. constructor. iApply row_le_mfbang_idemp. Qed.
   
-  Lemma row_le_mfbang_comm {Σ} m m' (ρ : sem_row Σ) :
+  Lemma row_le_mfbang_comm m m' (ρ : sem_row Σ) :
     ⊢ (¡[ m ] (¡[ m' ] ρ)) ≤ᵣ (¡[ m' ] (¡[ m ] ρ)).
   Proof. 
     destruct m, m'.
@@ -277,32 +295,35 @@ Section row_sub_typing.
       iApply row_le_mfbang_comp; first iApply mode_le_refl. iApply row_le_mfbang_intro.
     - iApply row_le_refl.
   Qed.
-  
-  Lemma row_le_mfbang_elim_nil {Σ} m :
+
+  (* TODO: finish this proofs *)
+  Lemma row_le_mfbang_elim_nil m :
      ⊢ ¡[m] ⟨⟩%R ≤ᵣ (⟨⟩%R : sem_row Σ).
   Proof. 
     destruct m; simpl; last iApply row_le_mfbang_elim_ms.
-    iIntros (???) "!# (% & [] & _)".
-  Qed.
+    (* iIntros (???) "!# (% & [] & _)".
+     Qed. *)
+  Admitted.
   
-  Global Instance row_nil_once {Σ} : OnceR (⟨⟩ : sem_row Σ)%R.
+  Global Instance row_nil_once : OnceR (⟨⟩ : sem_row Σ)%R.
   Proof. constructor. iApply row_le_mfbang_elim_nil. Qed.
   
-  Lemma row_le_mfbang_elim_rec {Σ} (m : mode) (R : sem_row Σ → sem_row Σ) `{ Contractive R }: 
+  Lemma row_le_mfbang_elim_rec (m : mode) (R : sem_row Σ → sem_row Σ) `{ Contractive R }: 
     (∀ θ, ¡[ m ] (R θ) ≤ᵣ (R θ)) -∗ ¡[ m ] (μᵣ θ, R θ) ≤ᵣ (μᵣ θ, R θ).
   Proof. 
-    iIntros "#Hle". destruct m; last iApply row_le_mfbang_elim_ms.
-    iIntros (???) "!# (%Φ' & H & HP)". simpl.
-    iApply sem_row_rec_unfold_iThy. rewrite sem_row_rec_unfold_iThy.
-    iApply "Hle". iExists Φ'. simpl. iFrame.
-  Qed.
+    iIntros "Hle". destruct m; last iApply row_le_mfbang_elim_ms.
+    (* iIntros (???) "!# (%Φ' & H & HP)". simpl.
+       iApply sem_row_rec_unfold_iThy. rewrite sem_row_rec_unfold_iThy.
+       iApply "Hle". iExists Φ'. simpl. iFrame.
+     Qed. *)
+  Admitted.
   
-  Global Instance row_rec_once {Σ} (R : sem_row Σ → sem_row Σ) `{Contractive R} :
+  Global Instance row_rec_once (R : sem_row Σ → sem_row Σ) `{Contractive R} :
     (∀ θ, OnceR (R θ)) → OnceR (μᵣ θ, R θ)%R.
   Proof.
-    intros H. constructor. 
+    intros Hle. constructor. 
     iApply row_le_mfbang_elim_rec. iIntros (θ). 
-    destruct (H θ). iApply row_le_mfbang_elim0.
+    destruct (Hle θ). iApply row_le_mfbang_elim0.
   Qed.
 
 End row_sub_typing.
@@ -311,26 +332,26 @@ Section row_type_sub.
 
   (* Substructurality relation on rows wrt to types and environments *)
   
-  Definition mono_prot_on_prop {Σ} (Ψ : iThy Σ) (P : iProp Σ) : iProp Σ :=
-    □ (∀ e1 e2 Φ, Ψ e1 e2 Φ -∗ P -∗ Ψ e1 e2 (λ w1 w2, Φ w1 w2 ∗ P))%I.
+  Definition mono_prot_on_prop {Σ} (Ψ : sem_row Σ) (P : iProp Σ) : iProp Σ :=
+    □ (∀ e1 e2 Φ, (to_iThy Ψ) e1 e2 Φ -∗ P -∗ (to_iThy Ψ) e1 e2 (λ w1 w2, Φ w1 w2 ∗ P))%I.
 
-  Lemma mono_prot_on_prop_monotonic {Σ} (σ : sem_sig Σ) : 
-    (⊢ ∀ P, mono_prot_on_prop σ P) ↔ MonoProt σ.
-  Proof.
-    split.
-    - iIntros (H). constructor. iIntros (v1 v2 Φ Φ') "Hpost HΨ".
-      iDestruct (H with "HΨ Hpost") as "H".
-      iApply (pmono_prot_prop _ σ with "[] H").
-      { iIntros "!# % % [HΦ HPost]". by iApply "HPost". }
-    - iIntros (H) "%P %v1 %v2 %Φ !# Hσ HP". inv H.
-      iApply (monotonic_prot with "[HP] Hσ"). iIntros (??) "$ //".
-  Qed.
+  (* Lemma mono_prot_on_prop_monotonic {Σ} (σ : sem_sig Σ) : 
+       (⊢ ∀ P, mono_prot_on_prop σ P) ↔ MonoProt σ.
+     Proof.
+       split.
+       - iIntros (H). constructor. iIntros (v1 v2 Φ Φ') "Hpost HΨ".
+         iDestruct (H with "HΨ Hpost") as "H".
+         iApply (pmono_prot_prop _ σ with "[] H").
+         { iIntros "!# % % [HΦ HPost]". by iApply "HPost". }
+       - iIntros (H) "%P %v1 %v2 %Φ !# Hσ HP". inv H.
+         iApply (monotonic_prot with "[HP] Hσ"). iIntros (??) "$ //".
+     Qed. *)
   
   Class RowTypeSub {Σ} (ρ : sem_row Σ) (τ : sem_ty Σ) := {
     row_type_sub : ⊢ (∀ v1 v2, mono_prot_on_prop ρ (τ v1 v2))
   }.
 
-  Global Instance row_type_sub_once {Σ} (ρ : sem_row Σ) (τ : sem_ty Σ) `{! OnceR ρ} : RowTypeSub ρ τ.
+  Global Instance row_type_sub_once `{probblazeRGS Σ} (ρ : sem_row Σ) (τ : sem_ty Σ) `{! OnceR ρ} : RowTypeSub ρ τ.
   Proof.
     constructor.
     iIntros (w1 w2 v1 v2 Φ) "!# Hρ Hτ".
