theories/prob_eff_lang/probblaze/sem_types.v
@@ -1,0 +1,387 @@
+(* sem_types.v *)
+
+(* This file contains the definition of semantic types *)
+
+From iris.proofmode Require Import base tactics.
+From iris.algebra Require Import ofe list.
+From iris.base_logic Require Export iprop upred invariants.
+
+(* Local imports *)
+From clutch.prob_eff_lang.probblaze Require Import logic notation sem_def mode sem_sig sem_row.
+
+(* Base types. *)
+Definition sem_ty_bot {Σ} : sem_ty Σ := (λ v1 v2, False)%I.
+
+Global Instance sem_ty_bot_instance {Σ} : Bottom (sem_ty Σ) := sem_ty_bot. 
+
+Definition sem_ty_unit {Σ} : sem_ty Σ := (λ v1 v2, ⌜ v1 = #()%V ∧ v2 = #()%V ⌝ )%I.
+Definition sem_ty_bool {Σ} : sem_ty Σ := (λ v1 v2, ∃ b : bool, ⌜ v1 = #b ∧ v2 = #b ⌝)%I.
+Definition sem_ty_nat {Σ} : sem_ty Σ := (λ v1 v2, ∃ n : nat, ⌜ v1 = #n ∧ v2 = #n ⌝)%I.
+Definition sem_ty_int {Σ} : sem_ty Σ := (λ v1 v2, ∃ n : Z, ⌜ v1 = #n ∧ v2 = #n ⌝)%I.
+Definition sem_ty_top {Σ} : sem_ty Σ := (λ v1 v2, True)%I.
+
+Global Instance sem_ty_top_instance {Σ} : Top (sem_ty Σ) := sem_ty_top. 
+Global Instance sem_ty_inhabited {Σ} : Inhabited (sem_ty Σ) := populate sem_ty_top. 
+
+Definition sem_ty_mbang {Σ} (m : mode) (τ : sem_ty Σ) : sem_ty Σ := (λ v1 v2, □? m (τ v1 v2))%I.
+
+Definition logN : namespace := nroot .@ "logN".
+(* Both tapes are empty and are sampled from the same distribution *)
+Definition sem_ty_tape `{probblazeGS Σ} : sem_ty Σ :=
+  (λ w1 w2,
+     ∃ (α1 α2 : loc) (N: nat), ⌜w1 = #lbl:α1⌝ ∧ ⌜w2 = #lbl:α2⌝ ∧
+                               inv (logN .@ (α1, α2)) (α1 ↪ (N; []) ∗ α2 ↪ₛ (N; [])))%I.
+
+(* Copyable Reference Type *)
+Definition tyN := nroot .@ "ty".
+Definition sem_ty_ref_cpy `{!probblazeGS Σ} (τ : sem_ty Σ): sem_ty Σ := 
+  (λ v1 v2, ∃ l1 l2 : loc, ⌜ v1 = #l1 ⌝ ∗ ⌜ v2 = #l2 ⌝ ∗ inv (tyN .@ (l1,l2)) (∃ w1 w2, l1 ↦ w1 ∗ l2 ↦ₛ w2 ∗ τ w1 w2))%I.
+
+(* Substructural Reference Type *)
+Definition sem_ty_ref `{!probblazeGS Σ} (τ : sem_ty Σ): sem_ty Σ := 
+  (λ v1 v2, ∃ l1 l2 : loc, ⌜ v1 = #l1 ⌝ ∗ ⌜ v2 = #l2 ⌝ ∗ (∃ w1 w2, l1 ↦ w1 ∗ l2 ↦ₛ w2 ∗ τ w1 w2))%I.
+
+(* Product type. *)
+Definition sem_ty_prod {Σ} (τ κ : sem_ty Σ) : sem_ty Σ := 
+  (λ v1 v2, ∃ w1 w1' w2 w2', ⌜v1 = (w1, w2)%V⌝ ∗ ⌜ v2 = (w1', w2')%V ⌝ ∗ τ w1 w1' ∗ κ w2 w2')%I.
+
+(* Sum type. *)
+Definition sem_ty_sum {Σ} (τ κ : sem_ty Σ) : sem_ty Σ :=
+  (λ v1 v2, ∃ w1 w2, (⌜v1 = InjLV w1%V⌝ ∗ ⌜v2 = InjLV w2%V⌝ ∗ τ w1 w2) ∨(⌜v1 = InjRV w1%V⌝ ∗ ⌜v2 = InjRV w2%V⌝ ∗ κ w1 w2))%I.
+
+(* Arrow type. *)
+Definition sem_ty_arr `{probblazeRGS Σ} 
+  (ρ : sem_row Σ)
+  (τ : sem_ty Σ)
+  (κ : sem_ty Σ) : sem_ty Σ :=
+  (λ (v1 v2 : val),
+    ∀ (w1 w2 : val),
+      τ w1 w2 -∗ BREL (v1 w1) ≤ (v2 w2) <| ρ |> {{ (λ u1 u2, κ u1 u2) }})%I.
+
+(* Polymorphic type. *)
+Definition sem_ty_type_forall {Σ} 
+  (C : sem_ty Σ → sem_ty Σ) : sem_ty Σ := (λ v1 v2, ∀ τ, C τ v1 v2)%I.
+
+(* Polymorphic effect type. *)
+Definition sem_ty_row_forall {Σ} 
+  (A : sem_row Σ → sem_ty Σ) : sem_ty Σ := (λ v1 v2, ∀ θ, A θ v1 v2)%I.
+
+(* Polymorphic mode type. *)
+Definition sem_ty_mode_forall {Σ} 
+  (C : mode → sem_ty Σ) : sem_ty Σ := (λ v1 v2, ∀ m, C m v1 v2)%I.
+
+(* Existential type. *)
+Definition sem_ty_exists `{probblazeGS Σ} 
+  (C : sem_ty Σ → sem_ty Σ) : sem_ty Σ := (λ v1 v2, ∃ τ, C τ v1 v2)%I.
+
+(** Recursive types *)
+Definition sem_ty_rec_pre {Σ} (C : sem_ty Σ → sem_ty Σ)
+  (rec : sem_ty Σ) : sem_ty Σ := (λ v1 v2, ▷ (∃ rec', rec ≡ rec' ∧ C rec' v1 v2))%I.
+Global Instance sem_ty_rec_pre_contractive {Σ} (C : sem_ty Σ → sem_ty Σ) :
+  Contractive (sem_ty_rec_pre C).
+Proof. solve_contractive. Qed.
+Definition sem_ty_rec {Σ} (C : sem_ty Σ -d> sem_ty Σ) : sem_ty Σ :=
+  fixpoint (sem_ty_rec_pre C).
+
+(* TODO: figure out the last part of the proof *)
+Lemma sem_ty_rec_unfold {Σ} (C : sem_ty Σ → sem_ty Σ) `{!NonExpansive C} v1 v2 :
+  (sem_ty_rec C)%T v1 v2 ⊣⊢ ▷ C (sem_ty_rec C)%T v1 v2. 
+Proof.
+  rewrite {1}/sem_ty_rec.
+  assert (fixpoint (sem_ty_rec_pre C) v1 v2 ≡ sem_ty_rec_pre C (fixpoint (sem_ty_rec_pre C)) v1 v2).
+  { do 2 apply non_dep_fun_equiv. apply fixpoint_unfold. }
+  rewrite H. iSplit.
+  - iIntros "(%rec' & #Hrec & HC) !>".
+      rewrite /sem_ty_rec.
+      iAssert (C rec' ≡ C (fixpoint (sem_ty_rec_pre C)))%I as "#H".
+      { by iRewrite "Hrec". }
+      rewrite !discrete_fun_equivI. (* iRewrite - ("H" $! v1). *) admit.
+  - iIntros "HC //=". iNext. iExists (sem_ty_rec C).
+    by iFrame. 
+Admitted.
+
+Notation "'𝟙'" := sem_ty_unit : sem_ty_scope.
+Notation "'𝔹'" := (sem_ty_bool) : sem_ty_scope.
+Notation "'ℤ'" := (sem_ty_int) : sem_ty_scope.
+Notation "![ m ] τ" := (sem_ty_mbang m τ) (at level 10) : sem_ty_scope.
+Notation "! τ" := (sem_ty_mbang MS τ) (at level 9, τ at level 9) : sem_ty_scope.
+
+Notation "τ '×' κ" := (sem_ty_prod τ%T κ%T) (at level 120) : sem_ty_scope.
+Infix "+" := (sem_ty_sum) : sem_ty_scope.
+
+Notation "'Ref' τ" := (sem_ty_ref τ%T) 
+  (at level 50) : sem_ty_scope.
+
+Notation "'Refᶜ' τ" := (sem_ty_ref_cpy τ%T) 
+  (at level 50) : sem_ty_scope.
+
+Notation "'∀ₜ' α , C " := (sem_ty_type_forall (λ α, C%T)) 
+  (at level 180) : sem_ty_scope.
+
+Notation "'∀ᵣ' θ , C " := (sem_ty_row_forall (λ θ, C%T)) 
+  (at level 180) : sem_ty_scope.
+
+Notation "'∀ₘ' ν , C " := (sem_ty_mode_forall (λ ν, C%T)) 
+  (at level 180) : sem_ty_scope.
+
+Notation "'∃ₜ' α , C " := (sem_ty_exists (λ α, C%T)) 
+  (at level 180) : sem_ty_scope.
+
+Notation "'μₜ' α , C " := (sem_ty_rec (λ α, C%T))
+  (at level 180) : sem_ty_scope.
+
+Notation "τ ⊸ κ" := (sem_ty_arr ⟨⟩%R τ%T κ%T)
+  (at level 99, κ at level 200) : sem_ty_scope.
+
+Notation "τ '-{' ρ '}-∘' κ" := (sem_ty_arr ρ%R τ%T κ%T)
+  (at level 100, ρ, κ at level 200) : sem_ty_scope.
+
+Notation "τ '-{' ρ '}-[' m ']->' κ" := (sem_ty_mbang m (sem_ty_arr ρ%R τ%T κ%T))%T
+  (at level 100, m, ρ, κ at level 200) : sem_ty_scope.
+
+Notation "τ '-[' m ']->' κ" := (sem_ty_mbang m (sem_ty_arr ⟨⟩%R τ%T κ%T))%T
+  (at level 100, m, κ at level 200) : sem_ty_scope.
+
+Notation "τ '-{' ρ '}->' κ" := (sem_ty_mbang MS (sem_ty_arr ρ%R τ%T κ%T))
+  (at level 100, ρ, κ at level 200) : sem_ty_scope.
+
+Notation "τ → κ" := (sem_ty_mbang MS (sem_ty_arr ⟨⟩%R τ%T κ%T))
+  (at level 99, κ at level 200) : sem_ty_scope.
+
+(* Derived Types *)
+Definition ListF {Σ} (τ : sem_ty Σ) := (λ α, 𝟙 + (τ × α))%T.
+
+(* List type. *)
+Definition sem_ty_list {Σ} (τ : sem_ty Σ) : sem_ty Σ := 
+    sem_ty_rec (ListF τ).
+
+Notation "'List' τ" := (sem_ty_list τ%T) 
+  (at level 50) : sem_ty_scope.
+
+(* List type. *)
+Definition sem_ty_option {Σ} (τ : sem_ty Σ) : sem_ty Σ := (𝟙 + τ)%T.
+
+Notation "'Option' τ" := (sem_ty_option τ%T) 
+  (at level 50) : sem_ty_scope.
+
+(**  Prove that type formers are non-expansive and respect setoid equality. *)
+Section types_properties.
+  Context `{probblazeRGS Σ}.
+
+  Implicit Types σ : sem_sig Σ.
+
+  Ltac solve_non_expansive :=
+    repeat intros ?;
+    unfold sem_ty_unit, sem_ty_int, sem_ty_bool, sem_ty_mbang,
+           sem_ty_prod, sem_ty_sum, sem_ty_arr,
+           sem_ty_ref, sem_ty_ref_cpy, 
+           sem_ty_rec, sem_ty_list, sem_ty_type_forall, sem_ty_exists;
+    repeat ( done || apply non_dep_fun_dist || intros ? || f_equiv).
+
+  Global Instance sem_ty_mbang_ne m : NonExpansive (@sem_ty_mbang Σ m).
+  Proof. solve_non_expansive. Qed.
+
+  Global Instance sem_ty_prod_ne : NonExpansive2 (@sem_ty_prod Σ).
+  Proof. solve_non_expansive. Qed.
+
+  Global Instance sem_ty_sum_ne : NonExpansive2 (@sem_ty_sum Σ).
+  Proof. solve_non_expansive. Qed.
+
+  Global Instance sem_ty_arr_ne : NonExpansive3 sem_ty_arr.
+  Proof. solve_non_expansive. Qed.
+
+  Global Instance sem_ty_ref_ne : NonExpansive (@sem_ty_ref Σ _).
+  Proof. solve_non_expansive. Qed.
+
+  Global Instance sem_ty_ref_cpy_ne : NonExpansive (@sem_ty_ref_cpy Σ _).
+  Proof. solve_non_expansive. Qed.
+
+  Global Instance sem_ty_type_forall_ne n :
+    Proper (pointwise_relation _ (dist n) ==> dist n) (@sem_ty_type_forall Σ).
+  Proof.
+    intros ?????. unfold sem_ty_type_forall; repeat f_equiv. 
+    by do 3apply non_dep_fun_dist.
+  Qed.
+
+  Global Instance sem_ty_type_forall_row_ne n :
+    Proper (pointwise_relation _ (dist n) ==> dist n) (@sem_ty_row_forall Σ).
+  Proof.
+    intros ?????. unfold sem_ty_row_forall; repeat f_equiv.
+    by do 2 apply non_dep_fun_dist.
+  Qed.
+
+  Global Instance sem_ty_type_forall_mode_ne n :
+    Proper (pointwise_relation _ (dist n) ==> dist n) (@sem_ty_mode_forall Σ).
+  Proof.
+    intros ?????. unfold sem_ty_mode_forall; repeat f_equiv. 
+    by do 2 apply non_dep_fun_dist.
+  Qed.
+
+  Global Instance sem_ty_exist_ne n :
+    Proper (pointwise_relation _ (dist n) ==> dist n) sem_ty_exists.
+  Proof. 
+    intros ?????. unfold sem_ty_exists; repeat f_equiv. 
+    by do 2 apply non_dep_fun_dist. 
+  Qed.
+
+  Global Instance sem_ty_rec_ne :
+    NonExpansive (@sem_ty_rec Σ).
+  Proof.
+    intros ????. unfold sem_ty_rec. apply fixpoint_ne.
+    intros ???. unfold sem_ty_rec_pre. do 4 f_equiv. 
+    by do 3 apply non_dep_fun_dist.
+  Qed.
+
+  Global Instance sem_ty_listF_ne τ : NonExpansive (@ListF Σ τ).
+  Proof. intros ?????. rewrite /ListF. 
+         apply non_dep_fun_dist. by repeat f_equiv.
+  Qed.
+
+  Global Instance sem_ty_listF_ne_2 : NonExpansive2 (@ListF Σ).
+  Proof. intros ???????. unfold ListF; by repeat f_equiv. Qed.
+
+  Global Instance sem_ty_list_ne : NonExpansive (@sem_ty_list Σ).
+  Proof. intros ?????. unfold sem_ty_list. 
+         apply non_dep_fun_dist. f_equiv. 
+         rewrite /ListF. intros ?. by repeat f_equiv.
+  Qed.
+  
+  Global Instance sem_ty_mbang_proper m : Proper ((≡) ==> (≡)) (@sem_ty_mbang Σ m).
+  (* Proof. solve_non_expansive. Qed. *)
+  Admitted.
+
+  Global Instance sem_ty_prod_proper : Proper ((≡) ==> (≡) ==> (≡)) (@sem_ty_prod Σ).
+  (* Proof. solve_non_expansive. Qed. *)
+  Admitted.
+
+  Global Instance sem_ty_sum_proper : Proper ((≡) ==> (≡) ==> (≡)) (@sem_ty_sum Σ).
+  (* Proof. solve_non_expansive. Qed. *)
+  Admitted.
+
+  Global Instance sem_ty_arr_proper : Proper ((≡) ==> (≡) ==> (≡) ==> (≡)) sem_ty_arr.
+  (* Proof. solve_non_expansive. Qed. *)
+  Admitted.
+
+  Global Instance sem_ty_ref_proper : Proper ((≡) ==> (≡)) (@sem_ty_ref Σ _).
+  (* Proof. intros ????. unfold sem_ty_ref; by repeat f_equiv. Qed. *)
+  Admitted.
+
+  Global Instance sem_ty_ref_cpy_proper : Proper ((≡) ==> (≡)) (@sem_ty_ref_cpy Σ _).
+  (* Proof. intros ????. unfold sem_ty_ref_cpy; by repeat f_equiv. Qed. *)
+  Admitted.
+
+  Global Instance sem_ty_type_forall_proper :
+    Proper (pointwise_relation _ (≡) ==> (≡)) (@sem_ty_type_forall Σ).
+  Proof. 
+    intros ?????. unfold sem_ty_type_forall; repeat f_equiv. 
+    by do 3 apply non_dep_fun_equiv. 
+  Qed.
+
+  Global Instance sem_ty_row_forall_proper :
+    Proper (pointwise_relation _ (≡) ==> (≡)) (@sem_ty_row_forall Σ).
+  Proof. 
+    intros ?????. unfold sem_ty_row_forall; repeat f_equiv. 
+    by do 3 apply non_dep_fun_equiv. 
+  Qed.
+
+  Global Instance sem_ty_mode_forall_proper :
+    Proper (pointwise_relation _ (≡) ==> (≡)) (@sem_ty_mode_forall Σ).
+  Proof. 
+    intros ?????. unfold sem_ty_mode_forall; repeat f_equiv. 
+    by do 3 apply non_dep_fun_equiv. 
+  Qed.
+
+  Global Instance sem_ty_exist_proper :
+    Proper (pointwise_relation _ (≡) ==>(≡)) sem_ty_exists.
+  Proof. 
+    intros ?????. unfold sem_ty_exists; repeat f_equiv.
+    by do 3 apply non_dep_fun_equiv.
+  Qed.
+
+  Global Instance sem_ty_rec_proper :
+    Proper (pointwise_relation _ (≡) ==>(≡)) (@sem_ty_rec Σ).
+  Proof.
+    intros C1 C2 HA. apply equiv_dist=> n.
+    apply sem_ty_rec_ne=> A. by apply equiv_dist.
+  Qed.
+
+  Global Instance sem_ty_mbang_persistent τ :
+    (∀ v1 v2, Persistent (@sem_ty_mbang Σ MS τ v1 v2)).
+  Proof. unfold sem_ty_mbang. simpl. apply _. Qed.
+
+  Global Instance sem_ty_type_forall_type_persistent (C : sem_ty Σ → sem_ty Σ) v1 v2 :
+    (∀ τ w1 w2, Persistent (C τ w1 w2)) →
+    Persistent ((sem_ty_type_forall C) v1 v2). 
+  Proof. unfold sem_ty_type_forall. simpl. apply _. Qed.
+
+  Global Instance sem_ty_row_forall_persistent (C : sem_row Σ → sem_ty Σ) v1 v2 :
+    (∀ τ w1 w2, Persistent (C τ w1 w2)) →
+    Persistent ((sem_ty_row_forall C) v1 v2).
+  Proof. unfold sem_ty_row_forall. simpl. apply _. Qed.
+
+  Global Instance sem_ty_mode_forall_persistent (C : mode → sem_ty Σ) v1 v2 :
+    (∀ τ w1 w2, Persistent (C τ w1 w2)) →
+    Persistent ((sem_ty_mode_forall C) v1 v2).
+  Proof. unfold sem_ty_mode_forall. simpl. apply _. Qed.
+
+End types_properties.
+
+Section multi_types.
+  
+  Context `{probblazeRGS Σ}.
+
+  Implicit Types τ κ : sem_ty Σ.
+  
+  Class MultiT {Σ} (τ : sem_ty Σ) := {
+    multi_ty : ⊢ (τ%T ≤ₜ ![MS] τ%T)
+  }.
+
+  Global Arguments MultiT _ _%_T.
+
+  Global Instance multi_ty_persistent (τ : sem_ty Σ) `{! MultiT τ} :
+    ∀ v1 v2, Persistent (τ v1 v2).
+  Proof. 
+    intros ??. inv MultiT0. 
+    rewrite /ty_le /tc_opaque /sem_ty_mbang /= in multi_ty0.
+    rewrite /Persistent. 
+    iIntros "Hτ.". iDestruct (multi_ty0 with "Hτ.") as "#Hτ".
+    by iModIntro.
+  Qed.
+
+End multi_types.
+
+Section sub_typing.
+
+  Context `{!probblazeRGS Σ}.
+
+  Implicit Types τ κ : sem_ty Σ.
+
+  Lemma ty_le_refl (τ : sem_ty Σ) : ⊢ τ ≤ₜ τ.
+  Proof. iIntros "!# % % $". Qed.
+
+  Lemma ty_le_trans (τ₁ τ₂ τ₃ : sem_ty Σ) :
+    τ₁ ≤ₜ τ₂ -∗
+    τ₂ ≤ₜ τ₃ -∗
+    τ₁ ≤ₜ τ₃.
+  Proof. 
+    iIntros "#Hτ₁₂ #Hτ₂₃ !# %v1 %v2 Hτ₁". 
+    iApply "Hτ₂₃". by iApply "Hτ₁₂".
+  Qed.
+
+  Lemma ty_le_bot (τ : sem_ty Σ) :
+    ⊢ ⊥ ≤ₜ τ.
+  Proof. iIntros "% % !# []". Qed.
+
+  (* Lemma ty_le_arr (τ₁ κ₁ τ₂ κ₂ : sem_ty Σ) (ρ ρ' : sem_row Σ) :
+       ρ ≤ᵣ ρ' -∗
+       τ₂ ≤ₜ τ₁ -∗
+       κ₁ ≤ₜ κ₂ -∗
+       (τ₁ -{ ρ }-∘ κ₁) ≤ₜ (τ₂ -{ ρ' }-∘ κ₂).
+     Proof.
+       iIntros "#Hρ  #Hτ₂₁ #Hκ₁₂ !# %v1 %v2 Hτκ₁". 
+       rewrite /sem_ty_arr /=. iIntros "% % Hτ₂".
+       iApply (ewpw_sub with "Hρ").
+       iApply (ewpw_mono with "[Hτκ₁ Hτ₂]").
+       { iApply ("Hτκ₁" with "[Hτ₂]"); by iApply "Hτ₂₁". }
+       iIntros "!# % Hκ !>". by iApply "Hκ₁₂".
+     Qed. *)
